Get rid of assn in the main theories!

Launchbury/Terms.thy
@@ -1,5 +1,5 @@
 theory Terms
-  imports "Nominal-Utils" Vars
+  imports "Nominal-Utils" Vars  "AList-Utils-Nominal"
 begin
 
 subsubsection {* Expressions *}
@@ -7,7 +7,7 @@ subsubsection {* Expressions *}
 nominal_datatype exp =
   Var "var"
 | App "exp" "var"
-| Let as::"assn" body::"exp" binds "bn as" in "body" "as"
+| LetA as::"assn" body::"exp" binds "bn as" in "body" "as"
 | Lam x::"var" body::"exp" binds x in body  ("Lam [_]. _" [100, 100] 100)
 and assn =
   ANil | ACons "var" "exp" "assn" 
@@ -17,15 +17,253 @@ where "bn ANil = []" | "bn (ACons x t as) = (atom x) # (bn as)"
 
 notation (latex output) Terms.Var ("_")
 notation (latex output) Terms.App ("_ _")
-notation (latex output) Terms.Let ("\<^raw:\textrm{\textsf{let}}> _ \<^raw:\textrm{\textsf{in}}> _")
+notation (latex output) Terms.LetA ("\<^raw:\textrm{\textsf{let}}> _ \<^raw:\textrm{\textsf{in}}> _")
 notation (latex output) Terms.Lam ("\<lambda>_. _"  [100, 100] 100)
 
 abbreviation
   LetBe :: "var\<Rightarrow>exp\<Rightarrow>exp\<Rightarrow>exp" ("let _ be _ in _ " [100,100,100] 100)
 where
-  "let x be t1 in t2 \<equiv> Let (ACons x t1 ANil) t2"
+  "let x be t1 in t2 \<equiv> LetA (ACons x t1 ANil) t2"
 
 type_synonym heap = "(var \<times> exp) list"
+
+subsubsection {* Rewriting in terms of heaps *}
+
+text {*
+The nominal package does not allow nested data types, hence the type @{type assn} above. But
+@{type assn} is isomorphic to @{type heap}, so at least now it should be possible to re-proof
+all resulting lemmas in terms of {@type heap}.
+*}
+
+subsubsection {* Conversion from assignments to heaps *}
+
+text {* The type @{typ assn} is the data type used in the let expression. It 
+is isomorphic to @{typ "(var \<times> exp) list"}, but since Nominal does not
+support nested data type, this redundancy was introduced. The following
+function converts between them. Once Nominal supports nested data types, this
+could be simplified. *}
+
+text {*
+Conversion from @{typ assn} to @{typ heap}.
+*}
+
+nominal_primrec asToHeap :: "assn \<Rightarrow> heap" 
+ where ANilToHeap: "asToHeap ANil = []"
+ | AConsToHeap: "asToHeap (ACons v e as) = (v, e) # asToHeap as"
+unfolding eqvt_def asToHeap_graph_aux_def
+apply rule
+apply simp
+apply rule
+apply(case_tac x rule: exp_assn.exhaust(2))
+apply auto
+done
+termination(eqvt) by lexicographic_order
+print_theorems
+
+lemma asToHeap_eqvt: "eqvt asToHeap"
+  unfolding eqvt_def
+  by (auto simp add: permute_fun_def asToHeap.eqvt)
+
+text {* The other direction. *}
+
+fun heapToAssn :: "heap \<Rightarrow> assn"
+  where "heapToAssn [] = ANil" 
+  | "heapToAssn ((v,e)#\<Gamma>) = ACons v e (heapToAssn \<Gamma>)"
+declare heapToAssn.simps[simp del]
+
+lemma heapToAssn_eqvt[simp,eqvt]: "p \<bullet> heapToAssn \<Gamma> =  heapToAssn (p \<bullet> \<Gamma>)"
+  by (induct \<Gamma> rule: heapToAssn.induct)
+     (auto simp add: heapToAssn.simps)
+
+lemma bn_heapToAssn: "bn (heapToAssn \<Gamma>) = map (\<lambda>x. atom (fst x)) \<Gamma>"
+  by (induct rule: heapToAssn.induct)
+     (auto simp add: heapToAssn.simps exp_assn.bn_defs)
+
+lemma set_bn_to_atom_domA:
+  "set (bn as) = atom ` domA (asToHeap as)"
+   by (induct as rule: asToHeap.induct)
+      (auto simp add: exp_assn.bn_defs)
+
+text {*
+They are inverse to each other.
+*}
+
+lemma heapToAssn_asToHeap[simp]:
+  "heapToAssn (asToHeap as) = as"
+  by (induct  rule: exp_assn.inducts(2)[of "\<lambda> _ . True"])
+     (auto simp add: heapToAssn.simps)
+
+lemma asToHeap_heapToAssn[simp]:
+  "asToHeap (heapToAssn as) = as"
+  by (induct rule: heapToAssn.induct)
+     (auto simp add: heapToAssn.simps)
+
+lemma heapToAssn_inject[simp]:
+  "heapToAssn x = heapToAssn y \<longleftrightarrow> x = y"
+  by (metis asToHeap_heapToAssn)
+
+lemma supp_heapToAssn: "supp (heapToAssn \<Gamma>) = supp \<Gamma>"
+  by (induct rule: heapToAssn.induct)
+     (simp_all add: heapToAssn.simps  exp_assn.supp supp_Nil supp_Cons supp_Pair sup_assoc)
+
+lemma supp_asToHeap: "supp (asToHeap as) = supp as"
+   by (induct as rule: asToHeap.induct)
+      (simp_all add:  exp_assn.supp supp_Nil supp_Cons supp_Pair sup_assoc)
+
+lemma fv_asToHeap: "fv (asToHeap \<Gamma>) = fv \<Gamma>"
+  unfolding fv_def by (auto simp add: supp_asToHeap)
+
+lemma fv_heapToAssn: "fv (heapToAssn \<Gamma>) = fv \<Gamma>"
+  unfolding fv_def by (auto simp add: supp_heapToAssn)
+
+lemma [simp]: "size (heapToAssn \<Gamma>) = list_size (\<lambda> (v,e) . size e) \<Gamma>"
+  by (induct rule: heapToAssn.induct)
+     (simp_all add: heapToAssn.simps)
+
+text {* The Let constructor that we are interested in. *}
+
+definition Let where "Let \<Gamma> e = LetA (heapToAssn \<Gamma>) e"
+notation (latex output) Terms.Let ("\<^raw:\textrm{\textsf{let}}> _ \<^raw:\textrm{\textsf{in}}> _")
+
+lemma size_Let[simp]: "size (Let \<Gamma> e) = list_size (\<lambda>p. size (snd p)) \<Gamma> + size e + Suc 0"
+  unfolding Let_def by (auto simp add: split_beta')
+
+text {*
+Now rewrite all (relevant) lemmas about @{term LetA} in terms of @{term LetB}.
+*}
+lemma Let_distinct[simp]:
+  "Var v \<noteq> Let \<Gamma> e"
+  "Let \<Gamma> e \<noteq> Var v"
+  "App e v \<noteq> Let \<Gamma> e'"
+  "Lam [v]. e' \<noteq> Let \<Gamma> e"
+  "Let \<Gamma> e \<noteq> Lam [v]. e'"
+  "Let \<Gamma> e' \<noteq> App e v"
+  unfolding Let_def by simp_all
+
+lemma Let_perm_simps[simp,eqvt]:
+  "p \<bullet> Let \<Gamma> e = Let (p \<bullet> \<Gamma>) (p \<bullet> e)"
+  unfolding Let_def by simp
+
+lemma Let_supp:
+  "supp (Let \<Gamma> e) = (supp e \<union> supp \<Gamma>) - atom ` (domA \<Gamma>)"
+  unfolding Let_def by (simp add: exp_assn.supp supp_heapToAssn bn_heapToAssn domA_def image_image)
+
+lemma Let_fresh[simp]:
+  "a \<sharp> Let \<Gamma> e = (a \<sharp> e \<and> a \<sharp> \<Gamma> \<or> a \<in> atom ` domA \<Gamma>)"
+  unfolding fresh_def by (auto simp add: Let_supp)
+
+lemma Abs_eq_cong:
+  assumes "\<And> p. (p \<bullet> x = x') \<longleftrightarrow> (p \<bullet> y = y')"
+  assumes "supp y = supp x"
+  assumes "supp y' = supp x'"
+  shows "([a]lst. x = [a']lst. x') \<longleftrightarrow> ([a]lst. y = [a']lst. y')"
+  by (simp add: Abs_eq_iff alpha_lst assms)
+
+
+lemma Let_eq_iff[simp]:
+  "(Let \<Gamma> e = Let \<Gamma>' e') = ([map (\<lambda>x. atom (fst x)) \<Gamma> ]lst. (e, \<Gamma>) = [map (\<lambda>x. atom (fst x)) \<Gamma>']lst. (e',\<Gamma>'))"
+  unfolding Let_def 
+  apply (simp add: bn_heapToAssn)
+  apply (rule Abs_eq_cong)
+  apply (simp_all add: supp_Pair supp_heapToAssn)
+  done
+
+lemma exp_strong_exhaust:
+  fixes c :: "'a :: fs"
+  assumes "(\<And>var. y = Var var \<Longrightarrow> P)"
+  assumes "\<And>exp var. y = App exp var \<Longrightarrow> P"
+  assumes "\<And>\<Gamma> exp. atom ` domA \<Gamma> \<sharp>* c \<Longrightarrow> y = Let \<Gamma> exp \<Longrightarrow> P"
+  assumes "\<And>var exp. {atom var} \<sharp>* c \<Longrightarrow> y = Lam [var]. exp \<Longrightarrow> P"
+  shows P
+  apply (rule  exp_assn.strong_exhaust(1)[where y = y and c = c])
+  apply (metis assms(1))
+  apply (metis assms(2))
+  apply (metis assms(3) set_bn_to_atom_domA Let_def heapToAssn_asToHeap)
+  apply (metis assms(4))
+  done
+
+text {*
+And finally the induction rules with @{term Let}.
+*}
+
+lemma exp_heap_induct[case_names Var App Let Lam Nil Cons]:
+  assumes "\<And>var. P1 (Var var)"
+  assumes "\<And>exp var. P1 exp \<Longrightarrow> P1 (App exp var)"
+  assumes "\<And>\<Gamma> exp. P2 \<Gamma> \<Longrightarrow> P1 exp \<Longrightarrow> P1 (Let \<Gamma> exp)"
+  assumes "\<And>var exp. P1 exp \<Longrightarrow> P1 (Lam [var]. exp)"
+  assumes "P2 []"
+  assumes "\<And>var exp \<Gamma>. P1 exp \<Longrightarrow> P2 \<Gamma> \<Longrightarrow> P2 ((var, exp)#\<Gamma>)"
+  shows "P1 e" and "P2 \<Gamma>"
+proof-
+  have "P1 e" and "P2 (asToHeap (heapToAssn \<Gamma>))"
+    apply (induct rule: exp_assn.inducts[of P1 "\<lambda> assn. P2 (asToHeap assn)"])
+    apply (metis assms(1))
+    apply (metis assms(2))
+    apply (metis assms(3) Let_def heapToAssn_asToHeap )
+    apply (metis assms(4))
+    apply (metis assms(5) asToHeap.simps(1))
+    apply (metis assms(6) asToHeap.simps(2))
+    done
+  thus "P1 e" and "P2 \<Gamma>" unfolding asToHeap_heapToAssn.
+qed
+
+lemma exp_heap_strong_induct[case_names Var App Let Lam Nil Cons]:
+  assumes "\<And>var c. P1 c (Var var)"
+  assumes "\<And>exp var c. (\<And>c. P1 c exp) \<Longrightarrow> P1 c (App exp var)"
+  assumes "\<And>\<Gamma> exp c. atom ` domA \<Gamma> \<sharp>* c \<Longrightarrow> (\<And>c. P2 c \<Gamma>) \<Longrightarrow> (\<And>c. P1 c exp) \<Longrightarrow> P1 c (Let \<Gamma> exp)"
+  assumes "\<And>var exp c. {atom var} \<sharp>* c \<Longrightarrow> (\<And>c. P1 c exp) \<Longrightarrow> P1 c (Lam [var]. exp)"
+  assumes "\<And>c. P2 c []"
+  assumes "\<And>var exp \<Gamma> c. (\<And>c. P1 c exp) \<Longrightarrow> (\<And>c. P2 c \<Gamma>) \<Longrightarrow> P2 c ((var,exp)#\<Gamma>)"
+  fixes c :: "'a :: fs"
+  shows "P1 c e" and "P2 c \<Gamma>"
+proof-
+  have "P1 c e" and "P2 c (asToHeap (heapToAssn \<Gamma>))"
+    apply (induct rule: exp_assn.strong_induct[of P1 "\<lambda> c assn. P2 c (asToHeap assn)"])
+    apply (metis assms(1))
+    apply (metis assms(2))
+    apply (metis assms(3) set_bn_to_atom_domA Let_def heapToAssn_asToHeap )
+    apply (metis assms(4))
+    apply (metis assms(5) asToHeap.simps(1))
+    apply (metis assms(6) asToHeap.simps(2))
+    done
+  thus "P1 c e" and "P2 c \<Gamma>" unfolding asToHeap_heapToAssn.
+qed
+
+subsubsection {* Nice induction rules *}
+
+text {*
+These rules can be used instead of the original induction rules, which require a separate
+goal for @{typ assn}.
+*}
+
+lemma exp_induct[case_names Var App Let Lam]:
+  assumes "\<And>var. P (Var var)"
+  assumes "\<And>exp var. P exp \<Longrightarrow> P (App exp var)"
+  assumes "\<And>\<Gamma> exp. (\<And> x. x \<in> domA \<Gamma> \<Longrightarrow>  P (the (map_of \<Gamma> x))) \<Longrightarrow> P exp \<Longrightarrow> P (Let \<Gamma> exp)"
+  assumes "\<And>var exp.  P exp \<Longrightarrow> P (Lam [var]. exp)"
+  shows "P  exp"
+  apply (rule exp_heap_induct[of P "\<lambda> \<Gamma>. (\<forall>x \<in> domA \<Gamma>. P (the (map_of \<Gamma> x)))"])
+  apply (metis assms(1))
+  apply (metis assms(2))
+  apply (metis assms(3))
+  apply (metis assms(4))
+  apply auto
+  done
+
+lemma  exp_strong_induct[case_names Var App Let Lam]:
+  assumes "\<And>var c. P c (Var var)"
+  assumes "\<And>exp var c. (\<And>c. P c exp) \<Longrightarrow> P c (App exp var)"
+  assumes "\<And>\<Gamma> exp c.
+    atom ` domA \<Gamma> \<sharp>* c \<Longrightarrow> (\<And>c x. x \<in> domA \<Gamma> \<Longrightarrow>  P c (the (map_of \<Gamma> x))) \<Longrightarrow> (\<And>c. P c exp) \<Longrightarrow> P c (Let \<Gamma> exp)"
+  assumes "\<And>var exp c. {atom var} \<sharp>* c \<Longrightarrow> (\<And>c. P c exp) \<Longrightarrow> P c (Lam [var]. exp)"
+  shows "P (c::'a::fs) exp"
+  apply (rule exp_heap_strong_induct(1)[of P "\<lambda> c \<Gamma>. (\<forall>x \<in> domA \<Gamma>. P c (the (map_of \<Gamma> x)))"])
+  apply (metis assms(1))
+  apply (metis assms(2))
+  apply (metis assms(3))
+  apply (metis assms(4))
+  apply auto
+  done
 
 subsubsection {* Testing alpha equivalence *}
               
@@ -39,11 +277,11 @@ lemma alpha_test2:
 
 lemma alpha_test3:
   shows "
-    Let (ACons x (Var y) (ACons y (Var x) ANil)) (Var x)
+    Let [(x, Var y), (y, Var x)] (Var x)
     =
-    Let (ACons y (Var x) (ACons x (Var y) ANil)) (Var y)" (is "Let ?la ?lb = _")
-  apply (simp add: exp_assn.bn_defs Abs1_eq_iff fresh_Pair add:fresh_at_base)
-  apply (simp add: Abs_swap2[of "atom x" "(?lb,?la)" "[atom x, atom y]" "atom y"])
+    Let [(y, Var x), (x, Var y)] (Var y)" (is "Let ?la ?lb = _")
+  apply (simp add: bn_heapToAssn Abs1_eq_iff fresh_Pair fresh_at_base)
+  apply (simp add: Abs_swap2[of "atom x" "(?lb, [(x, Var y), (y, Var x)])" "[atom x, atom y]" "atom y"])
 done
 
 subsubsection {* Free variables *}
@@ -52,15 +290,37 @@ lemma fv_supp_exp: "supp e = atom ` (fv (e::exp) :: var set)" and fv_supp_as: "s
   by (induction e and as rule:exp_assn.inducts)
      (auto simp add: fv_def exp_assn.supp supp_at_base)
 
+lemma fv_supp_heap: "supp (\<Gamma>::heap) = atom ` (fv \<Gamma> :: var set)"
+  by (metis fv_def fv_supp_as supp_heapToAssn)
+
 lemma fv_Lam[simp]: "fv (Lam [x]. e) = fv e - {x}"
   unfolding fv_def by (auto simp add: exp_assn.supp)
 lemma fv_Var[simp]: "fv (Var x) = {x}"
   unfolding fv_def by (auto simp add: exp_assn.supp supp_at_base)
 lemma fv_App[simp]: "fv (App e x) = insert x (fv e)"
   unfolding fv_def by (auto simp add: exp_assn.supp supp_at_base)
+lemma fv_Let[simp]: "fv (Let \<Gamma> e) = (fv \<Gamma> \<union> fv e) - domA \<Gamma>"
+  unfolding fv_def by (auto simp add: Let_supp exp_assn.supp supp_at_base set_bn_to_atom_domA)
+
+lemma finite_fv_exp[simp]: "finite (fv (e::exp) :: var set)"
+  and finite_fv_heap[simp]: "finite (fv (\<Gamma> :: heap) :: var set)"
+  by (induction e rule:exp_heap_induct) auto
 
 lemma fv_not_fresh: "atom x \<sharp> e \<longleftrightarrow> x \<notin> fv e"
   unfolding fv_def fresh_def by blast
+
+lemma fv_delete_heap:
+  assumes "map_of \<Gamma> x = Some e"
+  shows "fv (delete x \<Gamma>, e) \<union> {x} \<subseteq> (fv (\<Gamma>, Var x) :: var set)"
+proof-
+  have "fv (delete x \<Gamma>) \<subseteq> fv \<Gamma>" by (metis fv_delete_subset)
+  moreover
+  have "(x,e) \<in> set \<Gamma>" by (metis assms map_of_is_SomeD)
+  hence "fv e \<subseteq> fv \<Gamma>" by (metis assms domA_from_set map_of_fv_subset the.simps)
+  moreover
+  have "x \<in> fv (Var x)" by simp
+  ultimately show ?thesis by auto
+qed
 
 subsubsection {* Substitution *}
 
@@ -72,7 +332,18 @@ lemma subst_var_eqvts[eqvt]:
  shows "\<pi> \<bullet> (subst_var x y z) = subst_var (\<pi> \<bullet> x) (\<pi> \<bullet> y) (\<pi> \<bullet> z)"
 by auto
 
+
+lemma set_delete_subset: "set (delete x l) \<subseteq> set l"
+  by (induction l) auto
+
+(*
+lemma [simp]:"(a, b) \<in> set (\<Gamma>::heap) \<Longrightarrow> size b < Suc (list_size size \<Gamma> + size body)"
+  apply (induct \<Gamma> rule:heapToAssn.induct)
+  apply (auto simp add: exp_assn.bn_defs fresh_star_insert dest: set_mp[OF set_delete_subset])
+*)
+
 (* Helper lemmas provided by Christian Urban *)
+
 
 lemma Projl_permute:
   assumes a: "\<exists>y. f = Inl y"
@@ -85,32 +356,32 @@ lemma Projr_permute:
 using a by auto
 
 nominal_primrec  (default "sum_case (\<lambda>x. Inl undefined) (\<lambda>x. Inr undefined)",
-                  invariant "\<lambda> a r . (\<forall> as y z . ((a = Inr (as, y, z) \<and> set (bn as) \<sharp>* (y, z)) \<longrightarrow> bn (Sum_Type.Projr r) = bn as))")
+                  invariant "\<lambda> a r . (\<forall> as y z . ((a = Inr (as, y, z) \<and> atom ` domA as \<sharp>* (y, z)) \<longrightarrow> map (\<lambda>x . atom (fst x))  (Sum_Type.Projr r) = map (\<lambda>x . atom (fst x)) as))")
   subst :: "exp \<Rightarrow> var \<Rightarrow> var \<Rightarrow> exp" ("_[_::=_]" [1000,100,100] 1000)
 and
-  subst_assn :: "assn \<Rightarrow> var \<Rightarrow> var \<Rightarrow> assn" ("_[_::a=_]" [1000,100,100] 1000)
+  subst_heap :: "heap \<Rightarrow> var \<Rightarrow> var \<Rightarrow> heap" ("_[_::h=_]" [1000,100,100] 1000)
 where
   "(Var x)[y ::= z] = Var (x[y ::v= z])"
  |"(App e v)[y ::= z] = App (e[y ::= z]) (v[y ::v= z])"
- |"set (bn as) \<sharp>* (y,z) \<Longrightarrow> (Let as body)[y ::= z] = Let (as[y ::a= z]) (body[y ::= z])" 
+ |"atom ` domA as \<sharp>* (y,z) \<Longrightarrow> (Let as body)[y ::= z] = Let (as[y ::h= z]) (body[y ::= z])" 
  |"atom x \<sharp> (y,z) \<Longrightarrow> (Lam [x].e)[y ::= z] = Lam [x].(e[y::=z])"
- |"ANil[y ::a= z] = ANil"
- |"(ACons v e as)[y ::a= z] = ACons v (e[y ::= z]) (as[y ::a= z])"
+ |"[][y ::h= z] = []"
+ |"((v,e)# as)[y ::h= z] = (v, e[y ::= z])# (as[y ::h= z])"
 proof-
 
-have eqvt_at_subst: "\<And> e y z . eqvt_at subst_subst_assn_sumC (Inl (e, y, z)) \<Longrightarrow> eqvt_at (\<lambda>(a, b, c). subst a b c) (e, y, z)"
+have eqvt_at_subst: "\<And> e y z . eqvt_at subst_subst_heap_sumC (Inl (e, y, z)) \<Longrightarrow> eqvt_at (\<lambda>(a, b, c). subst a b c) (e, y, z)"
   apply(simp add: eqvt_at_def subst_def)
   apply(rule)
   apply(subst Projl_permute)
   apply(thin_tac "?X")+
-  apply (simp add: subst_subst_assn_sumC_def)
+  apply (simp add: subst_subst_heap_sumC_def)
   apply (simp add: THE_default_def)
-  apply (case_tac "Ex1 (subst_subst_assn_graph (Inl (e, y, z)))")
+  apply (case_tac "Ex1 (subst_subst_heap_graph (Inl (e, y, z)))")
   apply(simp)
   apply(auto)[1]
   apply (erule_tac x="x" in allE)
   apply simp
-  apply(cases rule: subst_subst_assn_graph.cases)
+  apply(cases rule: subst_subst_heap_graph.cases)
   apply(assumption)
   apply(rule_tac x="Sum_Type.Projl x" in exI)
   apply(clarify)
@@ -139,19 +410,19 @@ have eqvt_at_subst: "\<And> e y z . eqvt_at subst_subst_assn_sumC (Inl (e, y, z)
   apply(simp)
 done
 
-have eqvt_at_subst_assn: "\<And> as y z . eqvt_at subst_subst_assn_sumC (Inr (as, y, z)) \<Longrightarrow> eqvt_at (\<lambda>(a, b, c). subst_assn a b c) (as, y, z)"
-  apply(simp add: eqvt_at_def subst_assn_def)
+have eqvt_at_subst_heap: "\<And> as y z . eqvt_at subst_subst_heap_sumC (Inr (as, y, z)) \<Longrightarrow> eqvt_at (\<lambda>(a, b, c). subst_heap a b c) (as, y, z)"
+  apply(simp add: eqvt_at_def subst_heap_def)
   apply(rule)
   apply(subst Projr_permute)
   apply(thin_tac "?X")+
-  apply (simp add: subst_subst_assn_sumC_def)
+  apply (simp add: subst_subst_heap_sumC_def)
   apply (simp add: THE_default_def)
-  apply (case_tac "Ex1 (subst_subst_assn_graph (Inr (as, y, z)))")
+  apply (case_tac "Ex1 (subst_subst_heap_graph (Inr (as, y, z)))")
   apply(simp)
   apply(auto)[1]
   apply (erule_tac x="x" in allE)
   apply simp
-  apply(cases rule: subst_subst_assn_graph.cases)
+  apply(cases rule: subst_subst_heap_graph.cases)
   apply(assumption)
   apply (metis (mono_tags) Inr_not_Inl)+
   apply(rule_tac x="Sum_Type.Projr x" in exI)
@@ -174,12 +445,12 @@ done
 {
 (* Equivariance of the graph *)
 case goal1 thus ?case
-  unfolding eqvt_def subst_subst_assn_graph_aux_def
+  unfolding eqvt_def subst_subst_heap_graph_aux_def
   by simp
 
 (* The invariant *)
 next case goal2 thus ?case
-  by (induct rule: subst_subst_assn_graph.induct)(auto simp add: exp_assn.bn_defs fresh_star_insert)
+  by (induct rule: subst_subst_heap_graph.induct)(auto simp add: exp_assn.bn_defs fresh_star_insert)
 
 (* Exhaustiveness *)
 next case (goal3 P x) show ?case
@@ -188,7 +459,7 @@ next case (goal3 P x) show ?case
     proof(cases a)
     case (fields a1 a2 a3)
     thus P using Inl goal3
-      apply (rule_tac y ="a1" and c ="(a2, a3)" in exp_assn.strong_exhaust(1))
+      apply (rule_tac y ="a1" and c ="(a2, a3)" in exp_strong_exhaust)
       apply (auto simp add: fresh_star_def)
       apply metis
     done
@@ -198,29 +469,26 @@ next case (goal3 P x) show ?case
     proof (cases a)
     case (fields a1 a2 a3)
     thus P using Inr goal3
-      apply (rule_tac ya ="a1" in exp_assn.strong_exhaust(2))
-      apply (auto)
-      apply blast+
-    done
+      by (metis heapToAssn.cases)
   qed
 qed
 
 next case (goal15 e y2 z2 as e2 y z as2) thus ?case
   apply -
   apply (drule eqvt_at_subst)+
-  apply (drule eqvt_at_subst_assn)+
+  apply (drule eqvt_at_subst_heap)+
   apply (simp only: meta_eq_to_obj_eq[OF subst_def, symmetric, unfolded fun_eq_iff]
-    meta_eq_to_obj_eq[OF subst_assn_def, symmetric, unfolded fun_eq_iff])
+    meta_eq_to_obj_eq[OF subst_heap_def, symmetric, unfolded fun_eq_iff])
   (* No _sum any more at this point! *)
   apply (auto simp add: Abs_fresh_iff)
   apply (drule_tac
     c = "(y, z)" and
-    as = "(bn e)" and
-    bs = "(bn e2)" and
-    f = "\<lambda> a b c . [a]lst. (subst (fst b) y z, subst_assn (snd b) y z )" in Abs_lst_fcb2)
+    as = "(map (\<lambda>x. atom (fst x)) e)" and
+    bs = "(map (\<lambda>x. atom (fst x)) e2)" and
+    f = "\<lambda> a b c . [a]lst. (subst (fst b) y z, subst_heap (snd b) y z )" in Abs_lst_fcb2)
   apply (simp add: perm_supp_eq fresh_Pair fresh_star_def Abs_fresh_iff)
-  apply (simp)
-  apply (simp)
+  apply (metis domA_def image_image image_set)
+  apply (metis domA_def image_image image_set)
   apply (simp add: eqvt_at_def, simp add: fresh_star_Pair perm_supp_eq)
   apply (simp add: eqvt_at_def, simp add: fresh_star_Pair perm_supp_eq)
   apply (simp add: eqvt_at_def)
@@ -243,13 +511,13 @@ qed(auto)
 termination (eqvt) by lexicographic_order
 
 lemma shows
-  True and bn_subst[simp]: "set (bn as) \<sharp>* (y, z) \<Longrightarrow> bn (subst_assn as y z) = bn as"
-by(induct rule:subst_subst_assn.induct)
+  True and bn_subst[simp]: "domA (subst_heap as y z) = domA as"
+by(induct rule:subst_subst_heap.induct)
   (auto simp add: exp_assn.bn_defs fresh_star_insert)
 
 lemma subst_noop[simp]:
-shows "e[y ::= y] = e" and "as[y::a=y]= as"
-by(induct e y y and as y y rule:subst_subst_assn.induct)
+shows "e[y ::= y] = e" and "as[y::h=y]= as"
+by(induct e y y and as y y rule:subst_subst_heap.induct)
   (auto simp add:fresh_star_Pair exp_assn.bn_defs)
 
 lemma subst_is_fresh[simp]:
@@ -257,22 +525,22 @@ assumes "atom y \<sharp> z"
 shows
   "atom y \<sharp> e[y ::= z]"
 and
- "set (bn as) \<sharp>* y \<Longrightarrow> atom y \<sharp> as[y::a=z]"
+ "atom ` domA as \<sharp>* y \<Longrightarrow> atom y \<sharp> as[y::h=z]"
 using assms
-by(induct e y z and as y z rule:subst_subst_assn.induct)
-  (auto simp add:fresh_at_base fresh_star_Pair exp_assn.bn_defs fresh_star_insert)
+by(induct e y z and as y z rule:subst_subst_heap.induct)
+  (auto simp add:fresh_at_base fresh_star_Pair fresh_star_insert fresh_Nil fresh_Cons)
 
 lemma
  subst_pres_fresh: "x \<sharp> e \<Longrightarrow> x \<sharp> z \<Longrightarrow> x \<sharp> e[y ::= z]"
 and
- "x \<sharp> as \<Longrightarrow> x \<sharp> z \<Longrightarrow> x \<notin> set (bn as) \<Longrightarrow> x \<sharp> (as[y ::a= z])"
-by(induct e y z and as y z rule:subst_subst_assn.induct)
-  (auto simp add:fresh_star_Pair exp_assn.bn_defs)
+ "x \<sharp> \<Gamma> \<Longrightarrow> x \<sharp> z \<Longrightarrow> x \<notin> atom ` domA \<Gamma> \<Longrightarrow> x \<sharp> (\<Gamma>[y ::h= z])"
+by(induct e y z and \<Gamma> y z rule:subst_subst_heap.induct)
+  (auto simp add:fresh_star_Pair exp_assn.bn_defs fresh_Cons)
 
 lemma subst_fresh_noop: "atom x \<sharp> e \<Longrightarrow> e[x ::= y] = e"
-  and subst_assn_fresh_noop: "atom x \<sharp> as \<Longrightarrow> as[x ::a= y] = as"
-by (nominal_induct  e and as avoiding: x y rule:exp_assn.strong_induct)
-  (auto simp add: fresh_star_def fresh_Pair fresh_at_base simp del: exp_assn.eq_iff)
+  and subst_heap_fresh_noop: "atom x \<sharp> \<Gamma> \<Longrightarrow>  \<Gamma>[x ::h= y] = \<Gamma>"
+by (nominal_induct  e and \<Gamma> avoiding: x y rule:exp_heap_strong_induct)
+  (auto simp add: fresh_star_def fresh_Pair fresh_at_base fresh_Cons simp del: exp_assn.eq_iff)
 
 lemma supp_subst: "supp (e[y::=x]) \<subseteq> (supp e - {atom y}) \<union> supp x"
 proof-
@@ -297,13 +565,13 @@ lemma fresh_star_at_base:
   by (metis fresh_at_base(2) fresh_star_def)
 
 lemma subst_swap_same: "atom x \<sharp> e \<Longrightarrow>  (x \<leftrightarrow> y) \<bullet> e = e[y ::=x]"
-  and "atom x \<sharp> as \<Longrightarrow> set (bn as) \<sharp>* y \<Longrightarrow> (x \<leftrightarrow> y) \<bullet> as = as[y ::a= x]"
-by(nominal_induct  e and as avoiding: x y rule:exp_assn.strong_induct)
-  (auto simp add: fresh_star_Pair fresh_star_at_base exp_assn.bn_defs simp del: exp_assn.eq_iff)
+  and "atom x \<sharp> \<Gamma> \<Longrightarrow> atom `domA \<Gamma> \<sharp>* y \<Longrightarrow> (x \<leftrightarrow> y) \<bullet> \<Gamma> = \<Gamma>[y ::h= x]"
+by(nominal_induct  e and \<Gamma> avoiding: x y rule:exp_heap_strong_induct)
+  (auto simp add: fresh_star_Pair fresh_star_at_base fresh_Cons simp del: exp_assn.eq_iff)
 
 lemma subst_subst_back: "atom x \<sharp> e \<Longrightarrow>  e[y::=x][x::=y] = e" 
-  and "atom x \<sharp> as \<Longrightarrow> set (bn as) \<sharp>* y \<Longrightarrow> as[y::a=x][x::a=y] = as"
-by(nominal_induct  e and as avoiding: x y rule:exp_assn.strong_induct)
-  (auto simp add: fresh_star_Pair fresh_star_at_base  exp_assn.bn_defs simp del: exp_assn.eq_iff)
+  and "atom x \<sharp> \<Gamma> \<Longrightarrow> atom `domA \<Gamma> \<sharp>* y  \<Longrightarrow> \<Gamma>[y::h=x][x::h=y] = \<Gamma>"
+by(nominal_induct  e and \<Gamma> avoiding: x y rule:exp_heap_strong_induct)
+  (auto simp add: fresh_star_Pair fresh_star_at_base fresh_star_Cons fresh_Cons  exp_assn.bn_defs simp del: exp_assn.eq_iff)
 
 end
