Launchbury/CorrectnessOriginal.thy
@@ -139,37 +139,37 @@ next
 case (Let as \<Gamma> L body \<Delta> z)
   case 1
   { fix a
-    assume a: "a \<in> domA (asToHeap as)"
+    assume a: "a \<in> domA  as"
     have "atom a \<sharp> \<Gamma>" 
-      by (rule Let(1)[unfolded fresh_star_def set_bn_to_atom_domA, rule_format, OF imageI[OF a]])
+      by (rule Let(1)[unfolded fresh_star_def, rule_format, OF imageI[OF a]])
     hence "a \<notin> domA \<Gamma>"
       by (metis domA_not_fresh)
   }
   note * = this
 
   
-  have "fv (asToHeap as @ \<Gamma>, body) - domA (asToHeap as @ \<Gamma>) \<subseteq>  fv (\<Gamma>, Let as body) - domA \<Gamma>"
+  have "fv (as @ \<Gamma>, body) - domA (as @ \<Gamma>) \<subseteq>  fv (\<Gamma>, Let as body) - domA \<Gamma>"
     by auto
-  with 1 have prem: "fv (asToHeap as @ \<Gamma>, body) - domA (asToHeap as @ \<Gamma>) \<subseteq> set L" by auto
+  with 1 have prem: "fv (as @ \<Gamma>, body) - domA (as @ \<Gamma>) \<subseteq> set L" by auto
   
-  have f1: "atom ` domA (asToHeap as) \<sharp>* \<Gamma>"
+  have f1: "atom ` domA as \<sharp>* \<Gamma>"
     using Let(1) by (simp add: set_bn_to_atom_domA)
 
-  have "\<lbrakk> Let as body \<rbrakk>\<^bsub>\<lbrace>\<Gamma>\<rbrace>\<rho>\<^esub> = \<lbrakk> body \<rbrakk>\<^bsub>\<lbrace>asToHeap as\<rbrace>\<lbrace>\<Gamma>\<rbrace>\<rho>\<^esub>"
+  have "\<lbrakk> Let as body \<rbrakk>\<^bsub>\<lbrace>\<Gamma>\<rbrace>\<rho>\<^esub> = \<lbrakk> body \<rbrakk>\<^bsub>\<lbrace>as\<rbrace>\<lbrace>\<Gamma>\<rbrace>\<rho>\<^esub>"
     by (simp)
-  also have "\<dots> = \<lbrakk> body \<rbrakk>\<^bsub>\<lbrace>asToHeap as @ \<Gamma>\<rbrace>\<rho>\<^esub>"
+  also have "\<dots> = \<lbrakk> body \<rbrakk>\<^bsub>\<lbrace>as @ \<Gamma>\<rbrace>\<rho>\<^esub>"
     by (rule arg_cong[OF HSem_merge[OF f1]])
   also have "\<dots> = \<lbrakk> z \<rbrakk>\<^bsub>\<lbrace>\<Delta>\<rbrace>\<rho>\<^esub>"
     by (rule Let.hyps(4)[OF prem])
   finally
   show ?case.
 
-  have "(\<lbrace>\<Gamma>\<rbrace>\<rho>) f|` (domA \<Gamma>) = (\<lbrace>asToHeap as\<rbrace>(\<lbrace>\<Gamma>\<rbrace>\<rho>)) f|` (domA \<Gamma>)"
+  have "(\<lbrace>\<Gamma>\<rbrace>\<rho>) f|` (domA \<Gamma>) = (\<lbrace>as\<rbrace>(\<lbrace>\<Gamma>\<rbrace>\<rho>)) f|` (domA \<Gamma>)"
     apply (rule ext)
-    apply (case_tac "x \<in> domA (asToHeap as)")
+    apply (case_tac "x \<in> domA as")
     apply (auto simp add: lookup_HSem_other lookup_fmap_restr_eq *)
     done
-  also have "\<dots> = (\<lbrace>asToHeap as @ \<Gamma>\<rbrace>\<rho>) f|` (domA \<Gamma>)"
+  also have "\<dots> = (\<lbrace>as @ \<Gamma>\<rbrace>\<rho>) f|` (domA \<Gamma>)"
     by (rule arg_cong[OF HSem_merge[OF f1]])
   also have "\<dots> = (\<lbrace>\<Delta>\<rbrace>\<rho>) f|` (domA \<Gamma>)"
     by (rule fmap_restr_eq_subset[OF _ Let.hyps(5)[OF prem]]) simp
